pulse/share/steel/examples/pulse/dice/dpe/DPE.fsti
@@ -14,51 +14,9 @@ module U8 = FStar.UInt8
 module U32 = FStar.UInt32
 open Pulse.Lib.HashTable
 
-(* Engine Context *)
-noeq
-type engine_context = { uds: A.larray U8.t (US.v uds_len); }
 
-val engine_context_perm (c:engine_context) : vprop
-
-let mk_engine_context uds : engine_context = {uds}
-
-(* L0 Context *)
-noeq
-type l0_context = { cdi: A.larray U8.t (US.v dice_digest_len); }
-
-val l0_context_perm (c:l0_context) : vprop
-
-let mk_l0_context cdi : l0_context = {cdi}
-
-(* L1 Context *)
-noeq
-type l1_context = { deviceID_priv: A.larray U8.t (US.v v32us);
-                    deviceID_pub: A.larray U8.t (US.v v32us);
-                    aliasKey_priv: A.larray U8.t (US.v v32us);
-                    aliasKey_pub: A.larray U8.t (US.v v32us);
-                    aliasKeyCRT: A.array U8.t;
-                    deviceIDCSR: A.array U8.t; }
-
-val l1_context_perm (c:l1_context) : vprop
-
-let mk_l1_context deviceID_priv deviceID_pub aliasKey_priv aliasKey_pub aliasKeyCRT deviceIDCSR 
-  = { deviceID_priv; deviceID_pub; aliasKey_priv; aliasKey_pub; aliasKeyCRT; deviceIDCSR }
-
-(* Context *)
-noeq
-type context_t = 
-  | Engine_context : c:engine_context -> context_t
-  | L0_context     : c:l0_context -> context_t
-  | L1_context     : c:l1_context -> context_t
-
-val context_perm (t:context_t) : vprop
-
-let mk_engine_context_t engine_context = Engine_context engine_context
-let mk_l0_context_t l0_context = L0_context l0_context
-let mk_l1_context_t l1_context = L1_context l1_context
-
-let locked_context_t = c:context_t & L.lock (context_perm c)
-
+// hook this up to convert between wire format to pulse record
+// demo engine and l0 rec type
 
 (* Record *)
 noeq
@@ -74,43 +32,25 @@ type repr_t =
 val record_perm (t_rec:record_t) (t_rep:repr_t) : vprop
 
 
-type locked_ht_t (s:pht_sig_us) = ht:ht_t s & L.lock (exists_ (fun pht -> models s ht pht))
-type sid_ref_t = r:R.ref nat & L.lock (exists_ (fun n -> R.pts_to r full_perm n))
 
-val dpe_hashf : nat -> US.t
-val sht_len : pos_us
-val cht_len : pos_us
-let cht_sig : pht_sig_us = mk_pht_sig_us nat locked_context_t dpe_hashf
-let sht_sig : pht_sig_us = mk_pht_sig_us nat (locked_ht_t cht_sig) dpe_hashf 
 
-val locked_sht : locked_ht_t sht_sig
-val sid_ref : sid_ref_t
 
-val prng (_:unit) : nat
 
-val init_l0_ctxt (cdi:A.larray U8.t (US.v dice_digest_len)) (#s:erased (elseq U8.t dice_digest_len))
-  : stt locked_context_t
-    (A.pts_to cdi full_perm s ** pure (A.is_full_array cdi))
-    (fun _ -> A.pts_to cdi full_perm s)
+// return a session id 
+// use machine integers for sids and ctxt_hndl -- maybe make these abstract types
+val open_session (_:unit) : stt bool emp (fun _ -> emp)
 
-val init_l1_ctxt (deviceIDCSR_len: US.t) (aliasKeyCRT_len: US.t) 
-                (deviceID_priv: A.larray U8.t (US.v v32us)) (deviceID_pub: A.larray U8.t (US.v v32us))
-                (aliasKey_priv: A.larray U8.t (US.v v32us)) (aliasKey_pub: A.larray U8.t (US.v v32us)) 
-                (deviceIDCSR: A.larray U8.t (US.v deviceIDCSR_len)) (aliasKeyCRT: A.larray U8.t (US.v aliasKeyCRT_len))
-                (#s1 #s2 #s3 #s4: erased (elseq U8.t v32us)) 
-                (#s5:erased (elseq U8.t deviceIDCSR_len))
-                (#s6:erased (elseq U8.t aliasKeyCRT_len))
-  : stt locked_context_t
-     (A.pts_to deviceID_priv full_perm s1 ** 
-      A.pts_to deviceID_pub full_perm s2 **  
-      A.pts_to aliasKey_priv full_perm s3 **  
-      A.pts_to aliasKey_pub full_perm s4 **  
-      A.pts_to deviceIDCSR full_perm s5 ** 
-      A.pts_to aliasKeyCRT full_perm s6) 
-     (fun _ -> 
-      A.pts_to deviceID_priv full_perm s1 **  
-      A.pts_to deviceID_pub full_perm s2 ** 
-      A.pts_to aliasKey_priv full_perm s3 **  
-      A.pts_to aliasKey_pub full_perm s4 **  
-      A.pts_to deviceIDCSR full_perm s5 ** 
-      A.pts_to aliasKeyCRT full_perm s6)
+val destroy_context (sid:nat) (ctxt_hndl:nat) : stt bool emp (fun _ -> emp)
+
+val close_session (sid:nat) : stt bool emp (fun _ -> emp)
+
+// FIXME: dont need full perm on uds
+val initialize_context (sid:nat) (uds:A.larray U8.t (US.v uds_len))
+  : stt nat (A.pts_to uds full_perm uds_bytes ** 
+             uds_is_enabled **
+             pure (A.is_full_array uds))
+            (fun _ -> A.pts_to uds full_perm uds_bytes)
+
+val derive_child (sid:nat) (ctxt_hndl:nat) (record:record_t) (#repr:erased repr_t)
+  : stt nat (record_perm record repr) 
+            (fun _ -> record_perm record repr)
